Cleaned up parser theory

opentheory/theories/all.ml
@@ -151,9 +151,7 @@ loads "opentheory/theories/word16/word16.ml";;
 (* Stream parsers.                                                           *)
 (* ------------------------------------------------------------------------- *)
 
-(***
 loads "opentheory/theories/parser/parser.ml";;
-***)
 
 (* ------------------------------------------------------------------------- *)
 (* Unicode characters.                                                       *)
